sequiv is transitive

Transitivity.v
@@ -1,5 +1,50 @@
-Require Import Equivalence Reflexivity SessionTypes Tac Wellformed.
+Require Import Equivalence Reflexivity SessionTypes SessionTypesInd
+  Substitution SubstitutionFacts Tac Wellformed.
 
+Create HintDb trans discriminated.
+Hint Resolve sequiv_reflexive : trans.
+
+
+Inductive trans_helper : Sty -> Sty -> Prop :=
+| trans_helper_trans :
+    forall S T U,
+    wellformed S ->
+    wellformed T ->
+    wellformed U ->
+    sequiv S T ->
+    sequiv T U ->
+    trans_helper S U
+.
+Hint Constructors trans_helper : trans.
+
+Lemma trans_helper_refl :
+  forall S,
+  wellformed S ->
+  trans_helper S S.
+Proof. eauto with trans. Qed.
+
+Lemma sequiv_impl_trans_helper :
+  forall S T,
+  wellformed S ->
+  wellformed T ->
+  sequiv S T ->
+  trans_helper S T.
+Proof. eauto with trans. Qed.
+
+Lemma trans_helper_transitive :
+  (forall S T, trans_helper S T -> sequiv S T) ->
+  (forall S T U,
+    wellformed S ->
+    wellformed T ->
+    wellformed U ->
+    sequiv S T ->
+    sequiv T U ->
+    sequiv S U
+  ).
+Proof. eauto with trans. Qed.
+
+
+(* TODO beautify (a lot) *)
 Theorem sequiv_transitive :
   forall S T U,
   wellformed S ->
@@ -8,4 +53,105 @@ Theorem sequiv_transitive :
   sequiv S T ->
   sequiv T U ->
   sequiv S U.
-Proof. Admitted.
+Proof.
+  assert (
+    forall X S,
+    wellformed (mu X S) ->
+    wellformed (subst X (mu X S) S)
+  ) as L1 by skip.
+
+  apply trans_helper_transitive. apply sequiv_coind.
+  introv H. rename S' into U. inverts H.
+  assert (exists csT, cs T csT) as HcsT by eauto using cs_ex.
+  decompose_ex_auto.
+  assert (sequiv S csT) as HSeqT by (
+    eapply cs_preserves_sequiv_r with (S := S) (S' := T);
+    eauto using cs_preserves_sequiv_l
+  ).
+  assert (sequiv csT U) as HTeqU by (
+    eapply cs_preserves_sequiv_l with (S := T) (S' := U);
+    eauto using cs_preserves_sequiv_r
+  ).
+  clear H3 H4. inverts2 HSeqT; inverts2 HTeqU.
+
+  (* unit *)
+  - auto.
+
+  - constructor. apply sequiv_impl_trans_helper; auto.
+
+  (* send *)
+  - constructor. apply trans_helper_trans with (T := S'); eauto with wf.
+      assert (wellformed (send B S')) by
+        (eapply cs_preserves_wellformedness; eauto with wf).
+      eauto with wf.
+
+  - constructor. apply trans_helper_trans with (T := send B S'); eauto with wf.
+      eapply cs_preserves_wellformedness; eauto with wf.
+
+  (* recv *)
+  - constructor. apply trans_helper_trans with (T := S'); eauto with wf.
+      assert (wellformed (recv B S')) by
+        (eapply cs_preserves_wellformedness; eauto with wf).
+      eauto with wf.
+
+  - constructor. apply trans_helper_trans with (T := recv B S'); eauto with wf.
+      eapply cs_preserves_wellformedness; eauto with wf.
+
+  (* echoice *)
+  - assert (wellformed (echoice S1' S2')) by
+      (eapply cs_preserves_wellformedness; eauto with wf).
+    constructor.
+    * apply trans_helper_trans with (T := S1'); eauto with wf.
+    * apply trans_helper_trans with (T := S2'); eauto with wf.
+
+  - assert (wellformed (echoice S1' S2')) by
+      (eapply cs_preserves_wellformedness; eauto with wf).
+    constructor. apply trans_helper_trans with (T := echoice S1' S2');
+      eauto with wf.
+
+  (* ichoice *)
+  - assert (wellformed (ichoice S1' S2')) by
+      (eapply cs_preserves_wellformedness; eauto with wf).
+    constructor.
+    * apply trans_helper_trans with (T := S1'); eauto with wf.
+    * apply trans_helper_trans with (T := S2'); eauto with wf.
+
+  - assert (wellformed (ichoice S1' S2')) by
+      (eapply cs_preserves_wellformedness; eauto with wf).
+    constructor. apply trans_helper_trans with (T := ichoice S1' S2');
+      eauto with wf.
+
+  (* unit *)
+  - constructor. apply sequiv_impl_trans_helper; auto.
+
+  (* send *)
+  - constructor. apply trans_helper_trans with (T := send B S); auto.
+      eauto using cs_preserves_wellformedness with wf.
+
+  (* recv *)
+  - constructor. apply trans_helper_trans with (T := recv B S); auto.
+      eauto using cs_preserves_wellformedness with wf.
+
+  (* echoice *)
+  - constructor. apply trans_helper_trans with (T := echoice S1 S2); auto.
+      eauto using cs_preserves_wellformedness with wf.
+
+  (* ichoice *)
+  - constructor. apply trans_helper_trans with (T := ichoice S1 S2); auto.
+      eauto using cs_preserves_wellformedness with wf.
+
+  (* mu 1 (impossible) *)
+  - exfalso; eauto using cs_mu_absurd.
+
+  (* mu 2 *)
+  - constructor.
+    assert (sequiv csT (mu X0 S')) as HTeqU' by auto.
+    apply trans_helper_trans with (T := csT); eauto with wf.
+      eauto using cs_preserves_wellformedness.
+
+  (* mu 3 (impossible) *)
+  - exfalso; eauto using cs_mu_absurd.
+
+  (* mu 4 (impossible) *)
+  - exfalso; eauto using cs_mu_absurd.
+Qed.
